Classes: `Storable`, `ReadBytes`, `WriteBytes`

src/native/bytes_ref.c
@@ -1,8 +1,7 @@
 #include <string.h>
 #include "include/lean_pod.h"
-#include "util.h"
 
-LEAN_EXPORT lean_obj_res lean_pod_ByteArray_ref(lean_obj_arg ba, lean_obj_arg token) {
+LEAN_EXPORT lean_obj_res lean_pod_ByteArray_withRef(lean_obj_arg ba, lean_obj_arg f) {
     lean_object* resba;
     if(LEAN_LIKELY(lean_is_exclusive(ba))) {
         resba = ba;
@@ -11,7 +10,34 @@ LEAN_EXPORT lean_obj_res lean_pod_ByteArray_ref(lean_obj_arg ba, lean_obj_arg to
         resba = lean_copy_byte_array(ba);
         lean_dec_ref(ba);
     }
-    return lean_io_result_mk_ok(lean_pod_BytesView_wrap(lean_sarray_cptr(resba), resba));
+    lean_object* fres = lean_apply_2(f, lean_pod_BytesRef_wrap(lean_sarray_cptr(resba)), lean_box(0));
+    lean_dec_ref(fres);
+    return resba;
+}
+
+LEAN_EXPORT lean_obj_res lean_pod_ByteArray_withRefEx(lean_obj_arg ba, lean_obj_arg f) {
+    lean_object* resba;
+    if(LEAN_LIKELY(lean_is_exclusive(ba))) {
+        resba = ba;
+    }
+    else {
+        resba = lean_copy_byte_array(ba);
+        lean_dec_ref(ba);
+    }
+    lean_object* fres = lean_apply_2(f, lean_pod_BytesRef_wrap(lean_sarray_cptr(resba)), lean_box(0));
+    if(lean_ptr_tag(fres) == 1) {
+        lean_dec_ref(resba);
+        lean_object* exerr = lean_alloc_ctor(0, 1, 0);
+        lean_object* err = lean_ctor_get(fres, 0);
+        lean_inc(err);
+        lean_ctor_set(exerr, 0, err);
+        lean_dec_ref(fres);
+        return exerr;
+    }
+    lean_dec_ref(fres);
+    lean_object* exok = lean_alloc_ctor(1, 1, 0);
+    lean_ctor_set(exok, 0, resba);
+    return exok;
 }
 
 LEAN_EXPORT lean_obj_res lean_pod_BytesRef_weaken(uint8_t mut, size_t sz, b_lean_obj_arg a0, b_lean_obj_arg a1, lean_obj_arg bv) {
@@ -27,12 +53,13 @@ LEAN_EXPORT lean_obj_res lean_pod_BytesRef_take(uint8_t mut, size_t size, b_lean
 }
 
 LEAN_EXPORT lean_obj_res lean_pod_BytesRef_drop(uint8_t mut, size_t size, b_lean_obj_arg a, lean_obj_arg bv_w, size_t count) {
-    lean_pod_BytesView* bv = lean_pod_BytesView_unwrap(bv_w);
+    lean_pod_BytesRef br = lean_pod_BytesRef_unwrap(bv_w);
     if(lean_is_exclusive(bv_w)) {
-        bv->ptr += count;
+        lean_to_external(bv_w)->m_data = br + count;
         return bv_w;
     }
-    return lean_pod_BytesView_wrap(bv->ptr + count, bv->owner);
+    lean_dec_ref(bv_w);
+    return lean_pod_BytesRef_wrap(br + count);
 }
 
 LEAN_EXPORT lean_obj_res lean_pod_BytesRef_slice(uint8_t mut, size_t sz, b_lean_obj_arg a, lean_obj_arg bv_w, size_t start, size_t length) {
@@ -41,71 +68,6 @@ LEAN_EXPORT lean_obj_res lean_pod_BytesRef_slice(uint8_t mut, size_t sz, b_lean_
 
 LEAN_EXPORT lean_obj_res lean_pod_BytesRef_toByteArray(uint8_t mut, size_t sz, b_lean_obj_arg a, b_lean_obj_arg br, lean_obj_arg token) {
     lean_object* arr = lean_alloc_sarray(1, sz, sz);
-    memcpy(lean_sarray_cptr(arr), lean_pod_BytesView_unwrap(br)->ptr, sz);
+    memcpy(lean_sarray_cptr(arr), lean_pod_BytesRef_unwrap(br), sz);
     return lean_io_result_mk_ok(arr);
 }
-
-static inline lean_obj_res lean_pod_BytesRef_notStError() {
-    return lean_io_result_mk_ok(lean_panic_fn(
-        lean_box(0),
-        lean_mk_string("Error: `BytesRef` used in multithreaded context or while marked persistent")
-    ));
-}
-
-LEAN_EXPORT lean_obj_res lean_pod_BytesRef_getUInt8(uint8_t mut, size_t sz, b_lean_obj_arg a, b_lean_obj_arg br, size_t i, lean_obj_arg token) {
-    if (LEAN_LIKELY(lean_is_st(br))) {
-        return lean_io_result_mk_ok(lean_box(lean_pod_BytesView_unwrap(br)->ptr[i]));
-    }
-    return lean_pod_BytesRef_notStError();
-}
-
-LEAN_EXPORT lean_obj_res lean_pod_BytesRef_setUInt8(size_t sz, b_lean_obj_arg a, b_lean_obj_arg br, size_t i, uint8_t value, lean_obj_arg token) {
-    if (LEAN_LIKELY(lean_is_st(br))) {
-        lean_pod_BytesView_unwrap(br)->ptr[i] = value;
-        return lean_io_result_mk_ok(lean_box(0));
-    }
-    return lean_pod_BytesRef_notStError();
-}
-
-#define LEAN_POD_BYTESREF_GET_SET(bw, box)\
-LEAN_EXPORT lean_obj_res lean_pod_BytesRef_getUInt##bw##Ne(uint8_t mut, size_t sz, b_lean_obj_arg br, size_t i, lean_obj_arg token) {\
-    if (LEAN_LIKELY(lean_is_st(br))) {\
-        uint##bw##_t u;\
-        memcpy(&u, lean_pod_BytesView_unwrap(br)->ptr + i, sizeof(uint##bw##_t));\
-        return lean_io_result_mk_ok(box(u));\
-    }\
-    return lean_pod_BytesRef_notStError();\
-}\
-LEAN_EXPORT lean_obj_res LEAN_POD_CONCAT3(lean_pod_BytesRef_getUInt, bw, LEAN_POD_BYTESREF_E_KEEP)(uint8_t mut, size_t sz, b_lean_obj_arg br, size_t i, lean_obj_arg token) {\
-    return lean_pod_BytesRef_getUInt##bw##Ne(mut, sz, br, i, token);\
-}\
-LEAN_EXPORT lean_obj_res LEAN_POD_CONCAT3(lean_pod_BytesRef_getUInt, bw, LEAN_POD_BYTESREF_E_SWAP)(uint8_t mut, size_t sz, b_lean_obj_arg br, size_t i, lean_obj_arg token) {\
-    if (LEAN_LIKELY(lean_is_st(br))) {\
-        uint##bw##_t u;\
-        memcpy(&u, lean_pod_BytesView_unwrap(br)->ptr + i, sizeof(uint##bw##_t));\
-        return lean_io_result_mk_ok(box(lean_pod_bswap##bw(u)));\
-    }\
-    return lean_pod_BytesRef_notStError();\
-}\
-LEAN_EXPORT lean_obj_res lean_pod_BytesRef_setUInt##bw##Ne(size_t sz, b_lean_obj_arg br, size_t i, uint##bw##_t value, lean_obj_arg token) {\
-    if (LEAN_LIKELY(lean_is_st(br))) {\
-        memcpy(lean_pod_BytesView_unwrap(br)->ptr + i, &value, sizeof(uint##bw##_t));\
-        return lean_io_result_mk_ok(lean_box(0));\
-    }\
-    return lean_pod_BytesRef_notStError();\
-}\
-LEAN_EXPORT lean_obj_res LEAN_POD_CONCAT3(lean_pod_BytesRef_setUInt, bw, LEAN_POD_BYTESREF_E_KEEP)(size_t sz, b_lean_obj_arg br, size_t i, uint##bw##_t value, lean_obj_arg token) {\
-    return lean_pod_BytesRef_setUInt##bw##Ne(sz, br, i, value, token);\
-}\
-LEAN_EXPORT lean_obj_res LEAN_POD_CONCAT3(lean_pod_BytesRef_setUInt, bw, LEAN_POD_BYTESREF_E_SWAP)(size_t sz, b_lean_obj_arg br, size_t i, uint##bw##_t value, lean_obj_arg token) {\
-    if (LEAN_LIKELY(lean_is_st(br))) {\
-        uint##bw##_t value_bs = lean_pod_bswap##bw(value);\
-        memcpy(lean_pod_BytesView_unwrap(br)->ptr + i, &value_bs, sizeof(uint##bw##_t));\
-        return lean_io_result_mk_ok(lean_box(0));\
-    }\
-    return lean_pod_BytesRef_notStError();\
-}
-
-LEAN_POD_BYTESREF_GET_SET(16, lean_box);
-LEAN_POD_BYTESREF_GET_SET(32, lean_box_uint32);
-LEAN_POD_BYTESREF_GET_SET(64, lean_box_uint64);
