src/native/bytes_view.c
@@ -1,6 +1,5 @@
 #include <string.h>
 #include "include/lean_pod.h"
-#include "util.h"
 
 LEAN_EXPORT lean_obj_res lean_pod_ByteArray_view(lean_obj_arg ba) {
     return lean_pod_BytesView_wrap(lean_sarray_cptr(ba), ba);
@@ -20,6 +19,7 @@ LEAN_EXPORT lean_obj_res lean_pod_BytesView_drop(size_t size, b_lean_obj_arg a, 
         bv->ptr += count;
         return bv_w;
     }
+    lean_dec_ref(bv_w);
     return lean_pod_BytesView_wrap(bv->ptr + count, bv->owner);
 }
 
@@ -31,31 +31,4 @@ LEAN_EXPORT lean_obj_res lean_pod_BytesView_toByteArray(size_t sz, b_lean_obj_ar
     lean_object* arr = lean_alloc_sarray(1, sz, sz);
     memcpy(lean_sarray_cptr(arr), lean_pod_BytesView_unwrap(br)->ptr, sz);
     return arr;
-}
-
-LEAN_EXPORT uint8_t lean_pod_BytesView_getUInt8(size_t sz, b_lean_obj_arg a, b_lean_obj_arg bv, size_t i) {
-    return lean_pod_BytesView_unwrap(bv)->ptr[i];
-}
-
-#define LEAN_POD_BYTESVIEW_GET(bw)\
-LEAN_EXPORT uint##bw##_t lean_pod_BytesView_getUInt##bw##Ne(size_t sz, b_lean_obj_arg bv_w, size_t i) {\
-    uint##bw##_t u;\
-    memcpy(&u, lean_pod_BytesView_unwrap(bv_w)->ptr + i, sizeof(uint##bw##_t));\
-    return u;\
-}\
-LEAN_EXPORT uint##bw##_t LEAN_POD_CONCAT3(lean_pod_BytesView_getUInt,bw,LEAN_POD_BYTESREF_E_KEEP)(size_t sz, b_lean_obj_arg bv_w, size_t i) {\
-    return lean_pod_BytesView_getUInt##bw##Ne(sz, bv_w, i);\
-}\
-LEAN_EXPORT uint##bw##_t LEAN_POD_CONCAT3(lean_pod_BytesView_getUInt,bw,LEAN_POD_BYTESREF_E_SWAP)(size_t sz, b_lean_obj_arg bv_w, size_t i) {\
-    return lean_pod_bswap##bw(lean_pod_BytesView_getUInt##bw##Ne(sz, bv_w, i));\
-}
-
-LEAN_POD_BYTESVIEW_GET(16);
-LEAN_POD_BYTESVIEW_GET(32);
-LEAN_POD_BYTESVIEW_GET(64);
-
-LEAN_EXPORT size_t lean_pod_BytesView_getUSizeNe(size_t sz, b_lean_obj_arg bv, size_t i) {
-    size_t u;
-    memcpy(&u, lean_pod_BytesView_unwrap(bv)->ptr + i, sizeof(size_t));
-    return u;
 }
