src/native/endianness.c
@@ -1,0 +1,11 @@
+#include <lean/lean.h>
+
+LEAN_EXPORT uint8_t lean_pod_getEndianness(lean_obj_arg unit) {
+    #if __BYTE_ORDER__ == __ORDER_LITTLE_ENDIAN__
+        return 0;
+    #elif __BYTE_ORDER__ == __ORDER_BIG_ENDIAN__
+        return 1;
+    #else
+        #error unsupported
+    #endif
+}
