src/native/instances.c
@@ -1,0 +1,156 @@
+#include <string.h>
+#include "include/lean_pod.h"
+
+#if defined(__GNUC__) || defined(__clang__)
+#define LEAN_POD_ASSUME_ALIGNED(p, t) __builtin_assume_aligned(p, _Alignof(t))
+#else
+#define LEAN_POD_ASSUME_ALIGNED(p, t) p
+#endif
+
+static inline lean_obj_res lean_pod_BytesRef_notStError() {
+    return lean_io_result_mk_ok(lean_panic_fn(
+        lean_box(0),
+        lean_mk_string("Error: `BytesRef` used in multithreaded context or while marked persistent")
+    ));
+}
+
+#define LEAN_POD_RWBYTES_INST(ctyp, ltyp)\
+LEAN_EXPORT lean_obj_res lean_pod_readBytesRefUnal_##ltyp(b_lean_obj_arg a, b_lean_obj_arg br, lean_obj_arg st) {\
+    if (LEAN_LIKELY(lean_is_st(br))) {\
+        ctyp value;\
+        memcpy(&value, lean_pod_BytesRef_unwrap(br), sizeof(ctyp));\
+        return lean_io_result_mk_ok(lean_box(value));\
+    }\
+    return lean_pod_BytesRef_notStError();\
+}\
+LEAN_EXPORT lean_obj_res lean_pod_readBytesRefOffUnal_##ltyp(size_t sz, b_lean_obj_arg a, b_lean_obj_arg br, size_t i, lean_obj_arg st) {\
+    if (LEAN_LIKELY(lean_is_st(br))) {\
+        ctyp value;\
+        memcpy(&value, lean_pod_BytesRef_unwrap(br) + i, sizeof(ctyp));\
+        return lean_io_result_mk_ok(lean_box(value));\
+    }\
+    return lean_pod_BytesRef_notStError();\
+}\
+LEAN_EXPORT lean_obj_res lean_pod_readBytesRefOffElUnal_##ltyp(size_t sz, b_lean_obj_arg a, b_lean_obj_arg br, size_t i, lean_obj_arg st) {\
+    if (LEAN_LIKELY(lean_is_st(br))) {\
+        ctyp value;\
+        memcpy(&value, lean_pod_BytesRef_unwrap(br) + i * sizeof(ctyp), sizeof(ctyp));\
+        return lean_io_result_mk_ok(lean_box(value));\
+    }\
+    return lean_pod_BytesRef_notStError();\
+}\
+LEAN_EXPORT lean_obj_res lean_pod_readBytesRef_##ltyp(b_lean_obj_arg br, lean_obj_arg st) {\
+    if (LEAN_LIKELY(lean_is_st(br))) {\
+        ctyp value;\
+        char* p = lean_pod_BytesRef_unwrap(br);\
+        memcpy(&value, LEAN_POD_ASSUME_ALIGNED(p, ctyp), sizeof(ctyp));\
+        return lean_io_result_mk_ok(lean_box(value));\
+    }\
+    return lean_pod_BytesRef_notStError();\
+}\
+LEAN_EXPORT lean_obj_res lean_pod_readBytesRefOff_##ltyp(size_t sz, b_lean_obj_arg a, b_lean_obj_arg br, size_t i, lean_obj_arg st) {\
+    if (LEAN_LIKELY(lean_is_st(br))) {\
+        ctyp value;\
+        char* p = lean_pod_BytesRef_unwrap(br) + i;\
+        memcpy(&value, LEAN_POD_ASSUME_ALIGNED(p, ctyp), sizeof(ctyp));\
+        return lean_io_result_mk_ok(lean_box(value));\
+    }\
+    return lean_pod_BytesRef_notStError();\
+}\
+LEAN_EXPORT lean_obj_res lean_pod_readBytesRefOffEl_##ltyp(size_t sz, b_lean_obj_arg br, size_t i, lean_obj_arg st) {\
+    if (LEAN_LIKELY(lean_is_st(br))) {\
+        ctyp value;\
+        char* p = lean_pod_BytesRef_unwrap(br) + i * sizeof(ctyp);\
+        memcpy(&value, LEAN_POD_ASSUME_ALIGNED(p, ctyp), sizeof(ctyp));\
+        return lean_io_result_mk_ok(lean_box(value));\
+    }\
+    return lean_pod_BytesRef_notStError();\
+}\
+\
+LEAN_EXPORT ctyp lean_pod_readBytesViewUnal_##ltyp(b_lean_obj_arg a, b_lean_obj_arg bv) {\
+    ctyp value;\
+    memcpy(&value, lean_pod_BytesView_unwrap(bv)->ptr, sizeof(ctyp));\
+    return value;\
+}\
+LEAN_EXPORT ctyp lean_pod_readBytesViewOffUnal_##ltyp(size_t sz, b_lean_obj_arg a, b_lean_obj_arg bv, size_t i) {\
+    ctyp value;\
+    memcpy(&value, lean_pod_BytesView_unwrap(bv)->ptr + i, sizeof(ctyp));\
+    return value;\
+}\
+LEAN_EXPORT ctyp lean_pod_readBytesViewOffElUnal_##ltyp(size_t sz, b_lean_obj_arg a, b_lean_obj_arg bv, size_t i) {\
+    ctyp value;\
+    memcpy(&value, lean_pod_BytesView_unwrap(bv)->ptr + i * sizeof(ctyp), sizeof(ctyp));\
+    return value;\
+}\
+LEAN_EXPORT ctyp lean_pod_readBytesView_##ltyp(b_lean_obj_arg bv) {\
+    ctyp value;\
+    char* p = lean_pod_BytesView_unwrap(bv)->ptr;\
+    memcpy(&value, LEAN_POD_ASSUME_ALIGNED(p, ctyp), sizeof(ctyp));\
+    return value;\
+}\
+LEAN_EXPORT ctyp lean_pod_readBytesViewOff_##ltyp(size_t sz, b_lean_obj_arg a, b_lean_obj_arg bv, size_t i) {\
+    ctyp value;\
+    char* p = lean_pod_BytesView_unwrap(bv)->ptr + i;\
+    memcpy(&value, LEAN_POD_ASSUME_ALIGNED(p, ctyp), sizeof(ctyp));\
+    return value;\
+}\
+LEAN_EXPORT ctyp lean_pod_readBytesViewOffEl_##ltyp(size_t sz, b_lean_obj_arg bv, size_t i) {\
+    ctyp value;\
+    char* p = lean_pod_BytesView_unwrap(bv)->ptr + i * sizeof(ctyp);\
+    memcpy(&value, LEAN_POD_ASSUME_ALIGNED(p, ctyp), sizeof(ctyp));\
+    return value;\
+}\
+\
+LEAN_EXPORT lean_obj_res lean_pod_writeBytesRefUnal_##ltyp(b_lean_obj_arg a, b_lean_obj_arg br, ctyp value, lean_obj_arg st) {\
+    if (LEAN_LIKELY(lean_is_st(br))) {\
+        memcpy(lean_pod_BytesRef_unwrap(br), &value, sizeof(ctyp));\
+        return lean_io_result_mk_ok(lean_box(0));\
+    }\
+    return lean_pod_BytesRef_notStError();\
+}\
+LEAN_EXPORT lean_obj_res lean_pod_writeBytesRefOffUnal_##ltyp(size_t sz, b_lean_obj_arg a, b_lean_obj_arg br, size_t i, ctyp value, lean_obj_arg st) {\
+    if (LEAN_LIKELY(lean_is_st(br))) {\
+        memcpy(lean_pod_BytesRef_unwrap(br) + i, &value, sizeof(ctyp));\
+        return lean_io_result_mk_ok(lean_box(0));\
+    }\
+    return lean_pod_BytesRef_notStError();\
+}\
+LEAN_EXPORT lean_obj_res lean_pod_writeBytesRefOffElUnal_##ltyp(size_t sz, b_lean_obj_arg a, b_lean_obj_arg br, size_t i, ctyp value, lean_obj_arg st) {\
+    if (LEAN_LIKELY(lean_is_st(br))) {\
+        memcpy(lean_pod_BytesRef_unwrap(br) + i * sizeof(ctyp), &value, sizeof(ctyp));\
+        return lean_io_result_mk_ok(lean_box(0));\
+    }\
+    return lean_pod_BytesRef_notStError();\
+}\
+LEAN_EXPORT lean_obj_res lean_pod_writeBytesRef_##ltyp(b_lean_obj_arg br, ctyp value, lean_obj_arg st) {\
+    if (LEAN_LIKELY(lean_is_st(br))) {\
+        char* p = lean_pod_BytesRef_unwrap(br);\
+        memcpy(LEAN_POD_ASSUME_ALIGNED(p, ctyp), &value, sizeof(ctyp));\
+        return lean_io_result_mk_ok(lean_box(0));\
+    }\
+    return lean_pod_BytesRef_notStError();\
+}\
+LEAN_EXPORT lean_obj_res lean_pod_writeBytesRefOff_##ltyp(size_t sz, b_lean_obj_arg a, b_lean_obj_arg br, size_t i, ctyp value, lean_obj_arg st) {\
+    if (LEAN_LIKELY(lean_is_st(br))) {\
+        char* p = lean_pod_BytesRef_unwrap(br) + i;\
+        memcpy(LEAN_POD_ASSUME_ALIGNED(p, ctyp), &value, sizeof(ctyp));\
+        return lean_io_result_mk_ok(lean_box(0));\
+    }\
+    return lean_pod_BytesRef_notStError();\
+}\
+LEAN_EXPORT lean_obj_res lean_pod_writeBytesRefOffEl_##ltyp(size_t sz, b_lean_obj_arg br, size_t i, ctyp value, lean_obj_arg st) {\
+    if (LEAN_LIKELY(lean_is_st(br))) {\
+        char* p = lean_pod_BytesRef_unwrap(br) + i * sizeof(ctyp);\
+        memcpy(LEAN_POD_ASSUME_ALIGNED(p, ctyp), &value, sizeof(ctyp));\
+        return lean_io_result_mk_ok(lean_box(0));\
+    }\
+    return lean_pod_BytesRef_notStError();\
+}
+
+LEAN_POD_RWBYTES_INST(uint8_t, UInt8)
+LEAN_POD_RWBYTES_INST(uint16_t, UInt16)
+LEAN_POD_RWBYTES_INST(uint32_t, UInt32)
+LEAN_POD_RWBYTES_INST(uint64_t, UInt64)
+LEAN_POD_RWBYTES_INST(size_t, USize)
+LEAN_POD_RWBYTES_INST(double, Float)
+LEAN_POD_RWBYTES_INST(uint32_t, Float32)
