src/native/storable.c
@@ -1,0 +1,9 @@
+#include <lean/lean.h>
+
+LEAN_EXPORT lean_obj_res lean_pod_UInt64_getAlignment(b_lean_obj_arg unit) {
+    return lean_usize_to_nat(_Alignof(uint64_t));
+}
+
+LEAN_EXPORT lean_obj_res lean_pod_Float_getAlignment(b_lean_obj_arg unit) {
+    return lean_usize_to_nat(_Alignof(double));
+}
