src/lean/Pod/UInt.lean
@@ -20,25 +20,5 @@ def UInt64.bswap (value : UInt64) : UInt64 :=
   ((value &&& 0x000000000000FF00) <<< 40) |||
   ((value &&& 0x00000000000000FF) <<< 56)
 
-def UInt8.bitWidth : Nat := 8
-def UInt8.byteWidth : Nat := 1
-def UInt8.alignment : Nat := 1
-
-def UInt16.bitWidth : Nat := 16
-def UInt16.byteWidth : Nat := 2
-def UInt16.alignment : Nat := 2
-
-def UInt32.bitWidth : Nat := 32
-def UInt32.byteWidth : Nat := 4
-def UInt32.alignment : Nat := 4
-
-@[extern "lean_pod_UInt64_getAlignment"]
-opaque UInt64.getAlignment : @& Unit → { n : Nat // n = 4 ∨ n = 8 } := λ _ ↦ ⟨8, Or.inr rfl⟩
-
-def UInt64.bitWidth : Nat := 64
-def UInt64.byteWidth : Nat := 8
-def UInt64.alignment : Nat := UInt64.getAlignment ()
-
-def USize.bitWidth : Nat := System.Platform.numBits
-def USize.byteWidth : Nat := System.Platform.numBits / 8
-def USize.alignment : Nat := if System.Platform.numBits = 32 then 4 else 8
+@[extern "lean_pod_USize_bswap"]
+opaque USize.bswap (value : USize) : USize
