src/lean/Pod/BytesRef.lean
@@ -1,8 +1,5 @@
 import Pod.Lemmas
-import Pod.Util
 import Pod.UInt
-
-set_option autoImplicit false
 
 namespace Pod
 
@@ -24,13 +21,17 @@ abbrev BytesRefImm (σ : Type) := BytesRef σ .Immutable
 instance {size mutab align} : Nonempty (BytesRef σ mutab size align) := (BytesRefPointed σ mutab size align).property
 
 /-- Clones array if it is shared. -/
-@[extern "lean_pod_ByteArray_ref"]
-opaque _root_.ByteArray.ref (ba : ByteArray) : ST σ (BytesRefMut σ ba.size.toUSize 1)
+@[extern "lean_pod_ByteArray_withRef"]
+opaque _root_.ByteArray.withRef (ba : ByteArray) (f : BytesRefMut σ ba.size.toUSize 1 → ST σ Unit) : ByteArray
+
+/-- Clones array if it is shared. -/
+@[extern "lean_pod_ByteArray_withRefEx"]
+opaque _root_.ByteArray.withRefEx (ba : ByteArray) (f : BytesRefMut σ ba.size.toUSize 1 → EST ε σ Unit) : Except ε ByteArray
 
 namespace BytesRef
 
 @[extern "lean_pod_BytesRef_weaken"]
-opaque weaken {mutab size} {align0 align1 : @& Nat} (h : align1 ≤ align0) :
+opaque weaken {mutab size} {align0 align1 : @& Nat} (h : ∃ k, align1 * k = align0) :
   BytesRef σ mutab size align0 → BytesRef σ mutab size align1
 
 @[extern "lean_pod_BytesRef_imm"]
@@ -63,145 +64,5 @@ Read all bytes into a `ByteArray`.
 -/
 @[extern "lean_pod_BytesRef_toByteArray"]
 opaque toByteArray {mutab size} {align : @& Nat} (bv : @& BytesRef σ mutab size align) : ST σ ByteArray
-
-/--
-Read a `UInt8`.
-**Panics** when used in multithreaded context or if the `ByteRef` was marked persistent.
--/
-@[extern "lean_pod_BytesRef_getUInt8"]
-opaque getUInt8 {mutab size} {align : @& Nat} (bv : @& BytesRef σ mutab size align) (i : USize) (h : i < size) : ST σ UInt8
-
-/--
-Read a `UInt16` stored in native-endian order.
-**Panics** when used in multithreaded context or if the `ByteRef` was marked persistent.
--/
-@[extern "lean_pod_BytesRef_getUInt16Ne"]
-opaque getUInt16Ne {mutab size} (bv : @& BytesRef σ mutab size UInt16.alignment) (i : USize) (h : i + 1 < size) : ST σ UInt16
-
-/--
-Read a `UInt16` stored in little-endian order.
-**Panics** when used in multithreaded context or if the `ByteRef` was marked persistent.
--/
-@[extern "lean_pod_BytesRef_getUInt16Le"]
-opaque getUInt16Le {mutab size} (bv : @& BytesRef σ mutab size UInt16.alignment) (i : USize) (h : i + 1 < size) : ST σ UInt16
-
-/--
-Read a `UInt16` stored in big-endian order.
-**Panics** when used in multithreaded context or if the `ByteRef` was marked persistent.
--/
-@[extern "lean_pod_BytesRef_getUInt16Be"]
-opaque getUInt16Be {mutab size} (bv : @& BytesRef σ mutab size UInt16.alignment) (i : USize) (h : i + 1 < size) : ST σ UInt16
-
-/--
-Read a `UInt32` stored in native-endian order.
-**Panics** when used in multithreaded context or if the `ByteRef` was marked persistent.
--/
-@[extern "lean_pod_BytesRef_getUInt32Ne"]
-opaque getUInt32Ne {mutab size} (bv : @& BytesRef σ mutab size UInt32.alignment) (i : USize) (h : i + 3 < size) : ST σ UInt32
-
-/--
-Read a `UInt32` stored in little-endian order.
-**Panics** when used in multithreaded context or if the `ByteRef` was marked persistent.
--/
-@[extern "lean_pod_BytesRef_getUInt32Le"]
-opaque getUInt32Le {mutab size} (bv : @& BytesRef σ mutab size UInt32.alignment) (i : USize) (h : i + 3 < size) : ST σ UInt32
-
-/--
-Read a `UInt32` stored in big-endian order.
-**Panics** when used in multithreaded context or if the `ByteRef` was marked persistent.
--/
-@[extern "lean_pod_BytesRef_getUInt32Be"]
-opaque getUInt32Be {mutab size} (bv : @& BytesRef σ mutab size UInt32.alignment) (i : USize) (h : i + 3 < size) : ST σ UInt32
-
-/--
-Read a `UInt64` stored in native-endian order.
-**Panics** when used in multithreaded context or if the `ByteRef` was marked persistent.
--/
-@[extern "lean_pod_BytesRef_getUInt64Ne"]
-opaque getUInt64Ne {mutab size} (bv : @& BytesRef σ mutab size UInt64.alignment) (i : USize) (h : i + 7 < size) : ST σ UInt64
-
-/--
-Read a `UInt64` stored in little-endian order.
-**Panics** when used in multithreaded context or if the `ByteRef` was marked persistent.
--/
-@[extern "lean_pod_BytesRef_getUInt64Le"]
-opaque getUInt64Le {mutab size} (bv : @& BytesRef σ mutab size UInt64.alignment) (i : USize) (h : i + 7 < size) : ST σ UInt64
-
-/--
-Read a `UInt64` stored in big-endian order.
-**Panics** when used in multithreaded context or if the `ByteRef` was marked persistent.
--/
-@[extern "lean_pod_BytesRef_getUInt64Be"]
-opaque getUInt64Be {mutab size} (bv : @& BytesRef σ mutab size UInt64.alignment) (i : USize) (h : i + 7 < size) : ST σ UInt64
-
-/--
-Write to a `UInt8`.
-**Panics** when used in multithreaded context or if the `ByteRef` was marked persistent.
--/
-@[extern "lean_pod_BytesRef_setUInt8"]
-opaque setUInt8 {σ size align} (bv : @& BytesRefMut σ size align) (i : USize) (h : i < size) (value : UInt8) : ST σ Unit
-
-/--
-Write to a `UInt16` stored in native-endian order.
-**Panics** when used in multithreaded context or if the `ByteRef` was marked persistent.
--/
-@[extern "lean_pod_BytesRef_setUInt16Ne"]
-opaque setUInt16Ne {size} (bv : @& BytesRefMut σ size UInt16.alignment) (i : USize) (h : i + 1 < size) (value : UInt16) : ST σ Unit
-
-/--
-Write to a `UInt16` stored in little-endian order.
-**Panics** when used in multithreaded context or if the `ByteRef` was marked persistent.
--/
-@[extern "lean_pod_BytesRef_setUInt16Le"]
-opaque setUInt16Le {size} (bv : @& BytesRefMut σ size UInt16.alignment) (i : USize) (h : i + 1 < size) (value : UInt16) : ST σ Unit
-
-/--
-Write to a `UInt16` stored in big-endian order.
-**Panics** when used in multithreaded context or if the `ByteRef` was marked persistent.
--/
-@[extern "lean_pod_BytesRef_setUInt16Be"]
-opaque setUInt16Be {size} (bv : @& BytesRefMut σ size UInt16.alignment) (i : USize) (h : i + 1 < size) (value : UInt16) : ST σ Unit
-
-/--
-Write to a `UInt32` stored in native-endian order.
-**Panics** when used in multithreaded context or if the `ByteRef` was marked persistent.
--/
-@[extern "lean_pod_BytesRef_setUInt32Ne"]
-opaque setUInt32Ne {size} (bv : @& BytesRefMut σ size UInt32.alignment) (i : USize) (h : i + 3 < size) (value : UInt32) : ST σ Unit
-
-/--
-Write to a `UInt32` stored in little-endian order.
-**Panics** when used in multithreaded context or if the `ByteRef` was marked persistent.
--/
-@[extern "lean_pod_BytesRef_setUInt32Le"]
-opaque setUInt32Le {size} (bv : @& BytesRefMut σ size UInt32.alignment) (i : USize) (h : i + 3 < size) (value : UInt32) : ST σ Unit
-
-/--
-Write to a `UInt32` stored in big-endian order.
-**Panics** when used in multithreaded context or if the `ByteRef` was marked persistent.
--/
-@[extern "lean_pod_BytesRef_setUInt32Be"]
-opaque setUInt32Be {size} (bv : @& BytesRefMut σ size UInt32.alignment) (i : USize) (h : i + 3 < size) (value : UInt32) : ST σ Unit
-
-/--
-Write to a `UInt64` stored in native-endian order.
-**Panics** when used in multithreaded context or if the `ByteRef` was marked persistent.
--/
-@[extern "lean_pod_BytesRef_setUInt64Ne"]
-opaque setUInt64Ne {size} (bv : @& BytesRefMut σ size UInt64.alignment) (i : USize) (h : i + 7 < size) (value : UInt64) : ST σ Unit
-
-/--
-Write to a `UInt64` stored in little-endian order.
-**Panics** when used in multithreaded context or if the `ByteRef` was marked persistent.
--/
-@[extern "lean_pod_BytesRef_setUInt64Le"]
-opaque setUInt64Le {size} (bv : @& BytesRefMut σ size UInt64.alignment) (i : USize) (h : i + 7 < size) (value : UInt64) : ST σ Unit
-
-/--
-Write to a `UInt64` stored in big-endian order.
-**Panics** when used in multithreaded context or if the `ByteRef` was marked persistent.
--/
-@[extern "lean_pod_BytesRef_setUInt64Be"]
-opaque setUInt64Be {size} (bv : @& BytesRefMut σ size UInt64.alignment) (i : USize) (h : i + 7 < size) (value : UInt64) : ST σ Unit
 
 end Pod.BytesRef
