src/lean/Pod/BytesView.lean
@@ -1,5 +1,4 @@
 import Pod.Lemmas
-import Pod.Util
 import Pod.UInt
 
 namespace Pod
@@ -14,7 +13,7 @@ opaque _root_.ByteArray.view (ba : ByteArray) : BytesView ba.size.toUSize 1
 namespace BytesView
 
 @[extern "lean_pod_BytesView_weaken"]
-opaque weaken {size} {alignment0 alignment1 : @& Nat} (h : alignment1 ≤ alignment0) : BytesView size alignment0 → BytesView size alignment1
+opaque weaken {size} {alignment0 alignment1 : @& Nat} (h : ∃ k, alignment1 * k = alignment0) : BytesView size alignment0 → BytesView size alignment1
 
 @[extern "lean_pod_BytesView_take"]
 opaque take {size} {alignment : @& Nat} (bv : BytesView size alignment) (count : USize) (h : count ≤ size) : BytesView count alignment
@@ -39,82 +38,6 @@ opaque slice {size} {alignment : @& Nat}
 @[extern "lean_pod_BytesView_toByteArray"]
 opaque toByteArray {size} {align : @& Nat} (bv : @& BytesView size align) : ByteArray
 
-@[extern "lean_pod_BytesView_getUInt8"]
-opaque getUInt8 {size} {alignment : @& Nat} (bv : @& BytesView size alignment) (i : USize) (h : i < size) : UInt8
-
-@[extern "lean_pod_BytesView_getUInt16Ne"]
-opaque getUInt16Ne {size} (bv : @& BytesView size UInt16.alignment) (i : USize) (h : i + 1 < size) : UInt16
-
-@[extern "lean_pod_BytesView_getUInt16Le"]
-opaque getUInt16Le {size} (bv : @& BytesView size UInt16.alignment) (i : USize) (h : i + 1 < size) : UInt16
-
-@[extern "lean_pod_BytesView_getUInt16Be"]
-opaque getUInt16Be {size} (bv : @& BytesView size UInt16.alignment) (i : USize) (h : i + 1 < size) : UInt16
-
-@[extern "lean_pod_BytesView_getUInt32Ne"]
-opaque getUInt32Ne {size} (bv : @& BytesView size UInt32.alignment) (i : USize) (h : i + 3 < size) : UInt32
-
-@[extern "lean_pod_BytesView_getUInt32Le"]
-opaque getUInt32Le {size} (bv : @& BytesView size UInt32.alignment) (i : USize) (h : i + 3 < size) : UInt32
-
-@[extern "lean_pod_BytesView_getUInt32Be"]
-opaque getUInt32Be {size} (bv : @& BytesView size UInt32.alignment) (i : USize) (h : i + 3 < size) : UInt32
-
-@[extern "lean_pod_BytesView_getUInt64Ne"]
-opaque getUInt64Ne {size} (bv : @& BytesView size UInt64.alignment) (i : USize) (h : i + 7 < size) : UInt64
-
-@[extern "lean_pod_BytesView_getUInt64Le"]
-opaque getUInt64Le {size} (bv : @& BytesView size UInt64.alignment) (i : USize) (h : i + 7 < size) : UInt64
-
-@[extern "lean_pod_BytesView_getUInt64Be"]
-opaque getUInt64Be {size} (bv : @& BytesView size UInt64.alignment) (i : USize) (h : i + 7 < size) : UInt64
-
-@[extern "lean_pod_BytesView_getUSizeNe"]
-opaque getUSizeNe {size} (bv : @& BytesView size USize.alignment) (i : USize)
-  (h : i + (USize.byteWidth - 1).toUSize < size) : USize
-
-def getUInt8? {size alignment} (bv : BytesView size alignment) (i : USize) : Option UInt8 := mb? $ bv.getUInt8 i
-def getUInt16Ne? {size} (bv : BytesView size UInt16.alignment) (i : USize) : Option UInt16 := mb? $ bv.getUInt16Ne i
-def getUInt16Le? {size} (bv : BytesView size UInt16.alignment) (i : USize) : Option UInt16 := mb? $ bv.getUInt16Le i
-def getUInt16Be? {size} (bv : BytesView size UInt16.alignment) (i : USize) : Option UInt16 := mb? $ bv.getUInt16Be i
-def getUInt32Ne? {size} (bv : BytesView size UInt32.alignment) (i : USize) : Option UInt32 := mb? $ bv.getUInt32Ne i
-def getUInt32Le? {size} (bv : BytesView size UInt32.alignment) (i : USize) : Option UInt32 := mb? $ bv.getUInt32Le i
-def getUInt32Be? {size} (bv : BytesView size UInt32.alignment) (i : USize) : Option UInt32 := mb? $ bv.getUInt32Be i
-def getUInt64Ne? {size} (bv : BytesView size UInt64.alignment) (i : USize) : Option UInt64 := mb? $ bv.getUInt64Ne i
-def getUInt64Le? {size} (bv : BytesView size UInt64.alignment) (i : USize) : Option UInt64 := mb? $ bv.getUInt64Le i
-def getUInt64Be? {size} (bv : BytesView size UInt64.alignment) (i : USize) : Option UInt64 := mb? $ bv.getUInt64Be i
--- def getUSizeNe? {size} (bv : BytesView size USize.alignment) (i : USize) : Option USize :=
---   if h : 1 + (USize.byteWidth - 1).toUSize < size then some $ bv.getUSizeNe i h else none
-
-private
-abbrev mkGet! := @mb! "Index out of bounds"
-
-def getUInt8! {size alignment} (bv : BytesView size alignment) (i : USize) : UInt8 := mkGet! $ bv.getUInt8 i
-def getUInt16Ne! {size} (bv : BytesView size UInt16.alignment) (i : USize) : UInt16 := mkGet! $ bv.getUInt16Ne i
-def getUInt16Le! {size} (bv : BytesView size UInt16.alignment) (i : USize) : UInt16 := mkGet! $ bv.getUInt16Le i
-def getUInt16Be! {size} (bv : BytesView size UInt16.alignment) (i : USize) : UInt16 := mkGet! $ bv.getUInt16Be i
-def getUInt32Ne! {size} (bv : BytesView size UInt32.alignment) (i : USize) : UInt32 := mkGet! $ bv.getUInt32Ne i
-def getUInt32Le! {size} (bv : BytesView size UInt32.alignment) (i : USize) : UInt32 := mkGet! $ bv.getUInt32Le i
-def getUInt32Be! {size} (bv : BytesView size UInt32.alignment) (i : USize) : UInt32 := mkGet! $ bv.getUInt32Be i
-def getUInt64Ne! {size} (bv : BytesView size UInt64.alignment) (i : USize) : UInt64 := mkGet! $ bv.getUInt64Ne i
-def getUInt64Le! {size} (bv : BytesView size UInt64.alignment) (i : USize) : UInt64 := mkGet! $ bv.getUInt64Le i
-def getUInt64Be! {size} (bv : BytesView size UInt64.alignment) (i : USize) : UInt64 := mkGet! $ bv.getUInt64Be i
--- def getUSizeNe! {size} (bv : BytesView size USize.alignment) (i : USize) : USize := sorry
-
 end BytesView
 
 end Pod
-
-instance {size alignment} : GetElem (Pod.BytesView size alignment) USize UInt8 λ _ i ↦ i < size where
-  getElem := Pod.BytesView.getUInt8
-
-instance {size alignment} : GetElem (Pod.BytesView size alignment) Nat UInt8 λ _ i ↦ i < size.toNat where
-  getElem := λ bp i h ↦ bp.getUInt8 i.toUSize $ by
-    show i % USize.size < size.toNat
-    rw [Nat.mod_eq_of_lt $ Nat.lt_trans h size.val.isLt]
-    apply Nat.lt_of_lt_of_eq
-    · exact h
-    · rfl
-
-instance {size alignment} : GetElem (Pod.BytesView size alignment) (Fin size.toNat) UInt8 λ _ _ ↦ True where
-  getElem := λ bp i _ ↦ bp[i.val]'i.isLt
