src/lean/Pod/Endianness.lean
@@ -1,0 +1,11 @@
+namespace Pod
+
+inductive Endianness where
+  | LittleEndian
+  | BigEndian
+deriving Repr, Inhabited
+
+@[extern "lean_pod_getEndianness"]
+private opaque getEndianness : Unit → Endianness
+
+def endianness : Endianness := getEndianness ()
