src/lean/Pod/Instances.lean
@@ -1,0 +1,253 @@
+import Lean.Elab.Command
+import Pod.Lemmas
+import Pod.Float
+import Pod.Storable
+import Pod.ReadBytes
+import Pod.WriteBytes
+
+open Lean Syntax
+open Lean Elab Command
+
+namespace Pod
+
+section Instances
+
+set_option maxRecDepth 1024
+
+scoped elab "def_rwbytes_inst" typeName:str : command => do
+  let typeStr := typeName.getString
+  let typeId := mkIdent $ Name.mkSimple typeStr
+
+  let declStr := "readBytesRef_" ++ typeStr
+  let declName := Name.mkSimple $ declStr
+  let declName_rra0 := `Pod ++ declName
+  setEnv $ ← ofExcept $ externAttr.setParam (← getEnv) declName_rra0 $
+    ExternAttrData.mk none $ [ExternEntry.standard `all s!"lean_pod_{declStr}"]
+  Lean.Elab.Command.elabCommand $ ← `(command|
+    opaque $(mkIdent declName) {σ} (br : @& BytesRefImm σ (byteSize $typeId) (alignment $typeId)) : ST σ $typeId
+  )
+
+  let declStr := "readBytesRefOff_" ++ typeStr
+  let declName := Name.mkSimple $ declStr
+  let declName_rra1 := `Pod ++ declName
+  setEnv $ ← ofExcept $ externAttr.setParam (← getEnv) declName_rra1 $
+    ExternAttrData.mk none $ [ExternEntry.standard `all s!"lean_pod_{declStr}"]
+  Lean.Elab.Command.elabCommand $ ← `(command|
+    opaque $(mkIdent declName) {σ size} {align : @& Nat} (br : @& BytesRefImm σ size align) (i : USize)
+      (h₁ : i.toNat + (byteSize $typeId).toNat ≤ size.toNat)
+      (h₂ : ∀ m, ∃ n, align * m + i.toNat = (alignment $typeId) * n) : ST σ $typeId
+  )
+
+  let declStr := "readBytesRefOffEl_" ++ typeStr
+  let declName := Name.mkSimple $ declStr
+  let declName_rra2 := `Pod ++ declName
+  setEnv $ ← ofExcept $ externAttr.setParam (← getEnv) declName_rra2 $
+    ExternAttrData.mk none $ [ExternEntry.standard `all s!"lean_pod_{declStr}"]
+  Lean.Elab.Command.elabCommand $ ← `(command|
+    opaque $(mkIdent declName) {σ size} (br : @& BytesRefImm σ size (alignment $typeId)) (i : USize)
+      (h : i.toNat * (byteSize $typeId).toNat + (byteSize $typeId).toNat ≤ size.toNat) : ST σ $typeId
+  )
+
+  let declStr := "readBytesRefUnal_" ++ typeStr
+  let declName := Name.mkSimple $ declStr
+  let declName_rru0 := `Pod ++ declName
+  setEnv $ ← ofExcept $ externAttr.setParam (← getEnv) declName_rru0 $
+    ExternAttrData.mk none $ [ExternEntry.standard `all s!"lean_pod_{declStr}"]
+  Lean.Elab.Command.elabCommand $ ← `(command|
+    opaque $(mkIdent declName) {σ} {align : @& Nat} (br : @& BytesRefImm σ (byteSize $typeId) align) : ST σ $typeId
+  )
+
+  let declStr := "readBytesRefOffUnal_" ++ typeStr
+  let declName := Name.mkSimple $ declStr
+  let declName_rru1 := `Pod ++ declName
+  setEnv $ ← ofExcept $ externAttr.setParam (← getEnv) declName_rru1 $
+    ExternAttrData.mk none $ [ExternEntry.standard `all s!"lean_pod_{declStr}"]
+  Lean.Elab.Command.elabCommand $ ← `(command|
+    opaque $(mkIdent declName) {σ size} {align : @& Nat} (br : @& BytesRefImm σ size align) (i : USize)
+      (h₁ : i.toNat + (byteSize $typeId).toNat ≤ size.toNat) : ST σ $typeId
+  )
+
+  let declStr := "readBytesRefOffElUnal_" ++ typeStr
+  let declName := Name.mkSimple $ declStr
+  let declName_rru2 := `Pod ++ declName
+  setEnv $ ← ofExcept $ externAttr.setParam (← getEnv) declName_rru2 $
+    ExternAttrData.mk none $ [ExternEntry.standard `all s!"lean_pod_{declStr}"]
+  Lean.Elab.Command.elabCommand $ ← `(command|
+    opaque $(mkIdent declName) {σ size} {align : @& Nat} (br : @& BytesRefImm σ size align) (i : USize)
+      (h : i.toNat * (byteSize $typeId).toNat + (byteSize $typeId).toNat ≤ size.toNat) : ST σ $typeId
+  )
+
+  let declStr := "readBytesView_" ++ typeStr
+  let declName := Name.mkSimple $ declStr
+  let declName_va0 := `Pod ++ declName
+  setEnv $ ← ofExcept $ externAttr.setParam (← getEnv) declName_va0 $
+    ExternAttrData.mk none $ [ExternEntry.standard `all s!"lean_pod_{declStr}"]
+  Lean.Elab.Command.elabCommand $ ← `(command|
+    opaque $(mkIdent declName) (bv : @& BytesView (byteSize $typeId) (alignment $typeId)) : $typeId
+  )
+
+  let declStr := "readBytesViewOff_" ++ typeStr
+  let declName := Name.mkSimple $ declStr
+  let declName_va1 := `Pod ++ declName
+  setEnv $ ← ofExcept $ externAttr.setParam (← getEnv) declName_va1 $
+    ExternAttrData.mk none $ [ExternEntry.standard `all s!"lean_pod_{declStr}"]
+  Lean.Elab.Command.elabCommand $ ← `(command|
+    opaque $(mkIdent declName) {size} {align : @& Nat} (bv : @& BytesView size align) (i : USize)
+      (h₁ : i.toNat + (byteSize $typeId).toNat ≤ size.toNat)
+      (h₂ : ∀ m, ∃ n, align * m + i.toNat = (alignment $typeId) * n) : $typeId
+  )
+
+  let declStr := "readBytesViewOffEl_" ++ typeStr
+  let declName := Name.mkSimple $ declStr
+  let declName_va2 := `Pod ++ declName
+  setEnv $ ← ofExcept $ externAttr.setParam (← getEnv) declName_va2 $
+    ExternAttrData.mk none $ [ExternEntry.standard `all s!"lean_pod_{declStr}"]
+  Lean.Elab.Command.elabCommand $ ← `(command|
+    opaque $(mkIdent declName) {size} (bv : @& BytesView size (alignment $typeId)) (i : USize)
+      (h : i.toNat * (byteSize $typeId).toNat + (byteSize $typeId).toNat ≤ size.toNat) : $typeId
+  )
+
+  let declStr := "readBytesViewUnal_" ++ typeStr
+  let declName := Name.mkSimple $ declStr
+  let declName_vu0 := `Pod ++ declName
+  setEnv $ ← ofExcept $ externAttr.setParam (← getEnv) declName_vu0 $
+    ExternAttrData.mk none $ [ExternEntry.standard `all s!"lean_pod_{declStr}"]
+  Lean.Elab.Command.elabCommand $ ← `(command|
+    opaque $(mkIdent declName) {align : @& Nat} (bv : @& BytesView (byteSize $typeId) align) : $typeId
+  )
+
+  let declStr := "readBytesViewOffUnal_" ++ typeStr
+  let declName := Name.mkSimple $ declStr
+  let declName_vu1 := `Pod ++ declName
+  setEnv $ ← ofExcept $ externAttr.setParam (← getEnv) declName_vu1 $
+    ExternAttrData.mk none $ [ExternEntry.standard `all s!"lean_pod_{declStr}"]
+  Lean.Elab.Command.elabCommand $ ← `(command|
+    opaque $(mkIdent declName) {size} {align : @& Nat} (bv : @& BytesView size align) (i : USize)
+      (h₁ : i.toNat + (byteSize $typeId).toNat ≤ size.toNat) : $typeId
+  )
+
+  let declStr := "readBytesViewOffElUnal_" ++ typeStr
+  let declName := Name.mkSimple $ declStr
+  let declName_vu2 := `Pod ++ declName
+  setEnv $ ← ofExcept $ externAttr.setParam (← getEnv) declName_vu2 $
+    ExternAttrData.mk none $ [ExternEntry.standard `all s!"lean_pod_{declStr}"]
+  Lean.Elab.Command.elabCommand $ ← `(command|
+    opaque $(mkIdent declName) {size} {align : @& Nat} (bv : @& BytesView size align) (i : USize)
+      (h : i.toNat * (byteSize $typeId).toNat + (byteSize $typeId).toNat ≤ size.toNat) : $typeId
+  )
+
+  let declStr := "writeBytesRef_" ++ typeStr
+  let declName := Name.mkSimple $ declStr
+  let declName_rwa0 := `Pod ++ declName
+  setEnv $ ← ofExcept $ externAttr.setParam (← getEnv) declName_rwa0 $
+    ExternAttrData.mk none $ [ExternEntry.standard `all s!"lean_pod_{declStr}"]
+  Lean.Elab.Command.elabCommand $ ← `(command|
+    opaque $(mkIdent declName) {σ} (br : @& BytesRefMut σ (byteSize $typeId) (alignment $typeId))
+      (value : $typeId) : ST σ Unit
+  )
+
+  let declStr := "writeBytesRefOff_" ++ typeStr
+  let declName := Name.mkSimple $ declStr
+  let declName_rwa1 := `Pod ++ declName
+  setEnv $ ← ofExcept $ externAttr.setParam (← getEnv) declName_rwa1 $
+    ExternAttrData.mk none $ [ExternEntry.standard `all s!"lean_pod_{declStr}"]
+  Lean.Elab.Command.elabCommand $ ← `(command|
+    opaque $(mkIdent declName) {σ size} {align : @& Nat} (br : @& BytesRefMut σ size align) (i : USize)
+      (h₁ : i.toNat + (byteSize $typeId).toNat ≤ size.toNat)
+      (h₂ : ∀ m, ∃ n, align * m + i.toNat = (alignment $typeId) * n)
+      (value : $typeId) : ST σ Unit
+  )
+
+  let declStr := "writeBytesRefOffEl_" ++ typeStr
+  let declName := Name.mkSimple $ declStr
+  let declName_rwa2 := `Pod ++ declName
+  setEnv $ ← ofExcept $ externAttr.setParam (← getEnv) declName_rwa2 $
+    ExternAttrData.mk none $ [ExternEntry.standard `all s!"lean_pod_{declStr}"]
+  Lean.Elab.Command.elabCommand $ ← `(command|
+    opaque $(mkIdent declName) {σ size} (br : @& BytesRefMut σ size (alignment $typeId)) (i : USize)
+      (h : i.toNat * (byteSize $typeId).toNat + (byteSize $typeId).toNat ≤ size.toNat)
+      (value : $typeId) : ST σ Unit
+  )
+
+  let declStr := "writeBytesRefUnal_" ++ typeStr
+  let declName := Name.mkSimple $ declStr
+  let declName_rwu0 := `Pod ++ declName
+  setEnv $ ← ofExcept $ externAttr.setParam (← getEnv) declName_rwu0 $
+    ExternAttrData.mk none $ [ExternEntry.standard `all s!"lean_pod_{declStr}"]
+  Lean.Elab.Command.elabCommand $ ← `(command|
+    opaque $(mkIdent declName) {σ} {align : @& Nat} (br : @& BytesRefMut σ (byteSize $typeId) align)
+      (value : $typeId) : ST σ Unit
+  )
+
+  let declStr := "writeBytesRefOffUnal_" ++ typeStr
+  let declName := Name.mkSimple $ declStr
+  let declName_rwu1 := `Pod ++ declName
+  setEnv $ ← ofExcept $ externAttr.setParam (← getEnv) declName_rwu1 $
+    ExternAttrData.mk none $ [ExternEntry.standard `all s!"lean_pod_{declStr}"]
+  Lean.Elab.Command.elabCommand $ ← `(command|
+    opaque $(mkIdent declName) {σ size} {align : @& Nat} (br : @& BytesRefMut σ size align) (i : USize)
+      (h₁ : i.toNat + (byteSize $typeId).toNat ≤ size.toNat) (value : $typeId) : ST σ Unit
+  )
+
+  let declStr := "writeBytesRefOffElUnal_" ++ typeStr
+  let declName := Name.mkSimple $ declStr
+  let declName_rwu2 := `Pod ++ declName
+  setEnv $ ← ofExcept $ externAttr.setParam (← getEnv) declName_rwu2 $
+    ExternAttrData.mk none $ [ExternEntry.standard `all s!"lean_pod_{declStr}"]
+  Lean.Elab.Command.elabCommand $ ← `(command|
+    opaque $(mkIdent declName) {σ size} {align : @& Nat} (br : @& BytesRefMut σ size align) (i : USize)
+      (h : i.toNat * (byteSize $typeId).toNat + (byteSize $typeId).toNat ≤ size.toNat)
+      (value : $typeId) : ST σ Unit
+  )
+
+
+  Lean.Elab.Command.elabCommand $ ← `(command|
+    instance : ReadBytes $typeId where
+      readBytesRefOffUnal := $(mkIdent declName_rru1)
+      readBytesRefUnal := $(mkIdent declName_rru0)
+      readBytesRefOffElUnal := $(mkIdent declName_rru2)
+      readBytesRefOff := $(mkIdent declName_rra1)
+      readBytesRef := $(mkIdent declName_rra0)
+      readBytesRefOffEl := $(mkIdent declName_rra2)
+      readBytesViewOffUnal := $(mkIdent declName_vu1)
+      readBytesViewUnal := $(mkIdent declName_vu0)
+      readBytesViewOffElUnal := $(mkIdent declName_vu2)
+      readBytesViewOff := $(mkIdent declName_va1)
+      readBytesView := $(mkIdent declName_va0)
+      readBytesViewOffEl := $(mkIdent declName_va2)
+  )
+  Lean.Elab.Command.elabCommand $ ← `(command|
+    instance : WriteBytes $typeId where
+      writeBytesRefOffUnal := $(mkIdent declName_rwu1)
+      writeBytesRefUnal := $(mkIdent declName_rwu0)
+      writeBytesRefOffElUnal := $(mkIdent declName_rwu2)
+      writeBytesRefOff := $(mkIdent declName_rwa1)
+      writeBytesRef := $(mkIdent declName_rwa0)
+      writeBytesRefOffEl := $(mkIdent declName_rwa2)
+  )
+
+def_rwbytes_inst "UInt8"
+def_rwbytes_inst "UInt16"
+def_rwbytes_inst "UInt32"
+def_rwbytes_inst "UInt64"
+def_rwbytes_inst "USize"
+def_rwbytes_inst "Float"
+def_rwbytes_inst "Float32"
+
+instance {size alignment} : GetElem (Pod.BytesView size alignment) USize UInt8 λ _ i ↦ i < size where
+  getElem bv i h := Pod.readBytesViewOff_UInt8 bv i (by
+    show i.toNat + (1 % USize.size) ≤ size.toNat
+    rewrite [mod_usize_size_eq 1 (by decide)]
+    exact h
+  ) λ m ↦ Exists.intro (alignment * m + i.toNat) $ by
+    show alignment * m + i.toNat = 1 * (alignment * m + i.toNat)
+    rw [Nat.one_mul (alignment * m + i.toNat)]
+
+instance {size alignment} : GetElem (Pod.BytesView size alignment) Nat UInt8 λ _ i ↦ i < size.toNat where
+  getElem := λ bv i h ↦ bv[i.toUSize]'(by
+    show i % USize.size < size.toNat
+    rw [Nat.mod_eq_of_lt $ Nat.lt_trans h size.val.isLt]
+    apply Nat.lt_of_lt_of_eq
+    · exact h
+    · rfl
+  )
