src/lean/Pod/Lemmas.lean
@@ -1,4 +1,6 @@
-theorem Fin.toNat_sub_distrib {n} (a b : Fin n) (h : b ≤ a) :
+namespace Pod
+
+theorem _root_.Fin.toNat_sub_distrib {n} (a b : Fin n) (h : b ≤ a) :
   (a - b).val = a.val - b.val := by
   let aLt := a.isLt
   let a := a.val
@@ -16,3 +18,11 @@ theorem Fin.toNat_sub_distrib {n} (a b : Fin n) (h : b ≤ a) :
   apply Nat.lt_of_le_of_lt
   · exact Nat.sub_le a b
   · exact aLt
+
+theorem usize_size_ge_2_pow_32 : USize.size ≥ 2 ^ 32 :=
+  match usize_size_eq with
+    | Or.inl p => Nat.le_of_eq p.symm
+    | Or.inr p => Nat.le_of_lt $ Nat.lt_of_lt_of_eq (by decide) p.symm
+
+theorem mod_usize_size_eq (i : Nat) (h : i < 2^32) : i % USize.size = i :=
+  Nat.mod_eq_of_lt (Nat.lt_of_lt_of_le h usize_size_ge_2_pow_32)
