src/lean/Pod/ReadBytes.lean
@@ -1,0 +1,132 @@
+import Pod.Storable
+import Pod.BytesRef
+import Pod.BytesView
+
+namespace Pod
+
+class ReadBytes (α : Type) extends Storable α where
+  readBytesRefOffUnal {σ size align} : BytesRefImm σ size align → (i : USize) →
+    i.toNat + byteSize.toNat ≤ size.toNat → ST σ α
+
+  readBytesRefUnal {σ align} (br : BytesRefImm σ byteSize align) : ST σ α :=
+    readBytesRefOffUnal br 0 (Nat.le_of_eq $ Nat.zero_add _)
+
+  readBytesRefOffElUnal {σ size align} (br : BytesRefImm σ size align) (i : USize)
+    (h : i.toNat * byteSize.toNat + byteSize.toNat ≤ size.toNat) : ST σ α :=
+      readBytesRefOffUnal br (i * byteSize) (by rw [offEl_no_overflow i h]; exact h)
+
+  readBytesRefOff {σ size align} (br : BytesRefImm σ size align) (i : USize)
+    (h₁ : i.toNat + byteSize.toNat ≤ size.toNat)
+    (h₂ : (∀ m, ∃ n, align * m + i.toNat = alignment * n)) : ST σ α :=
+      readBytesRefOffUnal br i h₁
+
+  readBytesRef {σ} (br : BytesRefImm σ byteSize alignment) : ST σ α :=
+    readBytesRefOff br 0 (Nat.le_of_eq $ Nat.zero_add _) λ m ↦
+      Exists.intro m (by rw [Nat.add_comm]; exact Nat.zero_add _)
+
+  readBytesRefOffEl {σ size} (br : BytesRefImm σ size alignment) (i : USize)
+    (h : i.toNat * byteSize.toNat + byteSize.toNat ≤ size.toNat) : ST σ α :=
+      readBytesRefOff br (i * byteSize) (by rw [offEl_no_overflow i h]; exact h) (offEl_aligned i h)
+
+  readBytesViewOffUnal {size align} : BytesView size align → (i : USize) →
+    i.toNat + byteSize.toNat ≤ size.toNat → α
+
+  readBytesViewUnal {align} (bv : BytesView byteSize align) : α :=
+    readBytesViewOffUnal bv 0 (Nat.le_of_eq $ Nat.zero_add _)
+
+  readBytesViewOffElUnal {size align} (bv : BytesView size align)
+    (i : USize) (h : i.toNat * byteSize.toNat + byteSize.toNat ≤ size.toNat) : α :=
+      readBytesViewOffUnal bv (i * byteSize) (by rw [offEl_no_overflow i h]; exact h)
+
+  readBytesViewOff {size align} : BytesView size align → (i : USize) →
+    i.toNat + byteSize.toNat ≤ size.toNat →
+    (∀ m, ∃ n, align * m + i.toNat = alignment * n) → α
+
+  readBytesView (bv : BytesView byteSize alignment) : α :=
+    readBytesViewOff bv 0 (Nat.le_of_eq $ Nat.zero_add _) λ m ↦
+      Exists.intro m (by rw [Nat.add_comm]; exact Nat.zero_add _)
+
+  readBytesViewOffEl {size} (bv : BytesView size alignment)
+    (i : USize) (h : i.toNat * byteSize.toNat + byteSize.toNat ≤ size.toNat) : α :=
+      readBytesViewOff bv (i * byteSize) (by rw [offEl_no_overflow i h]; exact h) (offEl_aligned i h)
+
+
+def BytesRef.getUnal {α σ align} [ReadBytes α] (br : BytesRefImm σ (byteSize α) align) : ST σ α :=
+  ReadBytes.readBytesRefUnal br
+
+def BytesRef.ugetOffUnal {α σ size align} [ReadBytes α] (br : BytesRefImm σ size align) (i : USize)
+  (h₁ : i.toNat + (byteSize α).toNat ≤ size.toNat) : ST σ α :=
+    ReadBytes.readBytesRefOffUnal br i h₁
+
+def BytesRef.getOffUnal {α σ size align} [ReadBytes α] (br : BytesRefImm σ size align) (i : Nat)
+  (h₁ : i + (byteSize α).toNat ≤ size.toNat) : ST σ α :=
+    ReadBytes.readBytesRefOffUnal br ⟨i, off_lt_usize_size i h₁⟩ h₁
+
+def BytesRef.ugetOffElUnal {α σ size align} [ReadBytes α] (br : BytesRefImm σ size align)
+  (i : USize) (h : i.toNat * (byteSize α).toNat + (byteSize α).toNat ≤ size.toNat) : ST σ α :=
+    ReadBytes.readBytesRefOffElUnal br i h
+
+def BytesRef.getOffElUnal {α σ size align} [ReadBytes α] (br : BytesRefImm σ size align)
+  (i : Nat) (h : i * (byteSize α).toNat + (byteSize α).toNat ≤ size.toNat) : ST σ α :=
+    ReadBytes.readBytesRefOffElUnal br ⟨i, offEl_lt_usize_size i h⟩ h
+
+def BytesRef.get {α σ} [ReadBytes α] (br : BytesRefImm σ (byteSize α) (alignment α)) : ST σ α :=
+  ReadBytes.readBytesRef br
+
+def BytesRef.ugetOff {α σ size align} [ReadBytes α] (br : BytesRefImm σ size align) (i : USize)
+  (h₁ : i.toNat + (byteSize α).toNat ≤ size.toNat)
+  (h₂ : ∀ m, ∃ n, align * m + i.toNat = alignment α * n) : ST σ α :=
+    ReadBytes.readBytesRefOff br i h₁ h₂
+
+def BytesRef.getOff {α σ size align} [ReadBytes α] (br : BytesRefImm σ size align) (i : Nat)
+  (h₁ : i + (byteSize α).toNat ≤ size.toNat)
+  (h₂ : ∀ m, ∃ n, align * m + i = alignment α * n) : ST σ α :=
+    ReadBytes.readBytesRefOff br ⟨i, off_lt_usize_size i h₁⟩ h₁ h₂
+
+def BytesRef.ugetOffEl {α σ size} [ReadBytes α] (br : BytesRefImm σ size (alignment α))
+  (i : USize) (h : i.toNat * (byteSize α).toNat + (byteSize α).toNat ≤ size.toNat) : ST σ α :=
+    ReadBytes.readBytesRefOffEl br i h
+
+def BytesRef.getOffEl {α σ size} [ReadBytes α] (br : BytesRefImm σ size (alignment α))
+  (i : Nat) (h : i * (byteSize α).toNat + (byteSize α).toNat ≤ size.toNat) : ST σ α :=
+    ReadBytes.readBytesRefOffEl br ⟨i, offEl_lt_usize_size i h⟩ h
+
+def BytesView.getUnal {α align} [ReadBytes α] (bv : BytesView (byteSize α) align) : α :=
+  ReadBytes.readBytesViewUnal bv
+
+def BytesView.ugetOffUnal {α size align} [ReadBytes α] (bv : BytesView size align) (i : USize)
+  (h₁ : i.toNat + (byteSize α).toNat ≤ size.toNat) : α :=
+    ReadBytes.readBytesViewOffUnal bv i h₁
+
+def BytesView.getOffUnal {α size align} [ReadBytes α] (bv : BytesView size align) (i : Nat)
+  (h₁ : i + (byteSize α).toNat ≤ size.toNat) : α :=
+    ReadBytes.readBytesViewOffUnal bv ⟨i, off_lt_usize_size i h₁⟩ h₁
+
+def BytesView.ugetOffElUnal {α size align} [ReadBytes α] (bv : BytesView size align)
+  (i : USize) (h : i.toNat * (byteSize α).toNat + (byteSize α).toNat ≤ size.toNat) : α :=
+    ReadBytes.readBytesViewOffElUnal bv i h
+
+def BytesView.getOffElUnal {α size align} [ReadBytes α] (bv : BytesView size align)
+  (i : Nat) (h : i * (byteSize α).toNat + (byteSize α).toNat ≤ size.toNat) : α :=
+    ReadBytes.readBytesViewOffElUnal bv ⟨i, offEl_lt_usize_size i h⟩ h
+
+def BytesView.get {α} [ReadBytes α] (bv : BytesView (byteSize α) (alignment α)) : α :=
+  ReadBytes.readBytesView bv
+
+def BytesView.ugetOff {α size align} [ReadBytes α] (bv : BytesView size align) (i : USize)
+  (h₁ : i.toNat + (byteSize α).toNat ≤ size.toNat)
+  (h₂ : ∀ m, ∃ n, align * m + i.toNat = alignment α * n) : α :=
+    ReadBytes.readBytesViewOff bv i h₁ h₂
+
+def BytesView.getOff {α size align} [ReadBytes α] (bv : BytesView size align) (i : Nat)
+  (h₁ : i + (byteSize α).toNat ≤ size.toNat)
+  (h₂ : ∀ m, ∃ n, align * m + i = alignment α * n) : α :=
+    ReadBytes.readBytesViewOff bv ⟨i, off_lt_usize_size i h₁⟩ h₁ h₂
+
+def BytesView.ugetOffEl {α size} [ReadBytes α] (bv : BytesView size (alignment α))
+  (i : USize) (h : i.toNat * (byteSize α).toNat + (byteSize α).toNat ≤ size.toNat) : α :=
+    ReadBytes.readBytesViewOffEl bv i h
+
+def BytesView.getOffEl {α size} [ReadBytes α] (bv : BytesView size (alignment α))
+  (i : Nat) (h : i * (byteSize α).toNat + (byteSize α).toNat ≤ size.toNat) : α :=
+    ReadBytes.readBytesViewOffEl bv ⟨i, offEl_lt_usize_size i h⟩ h
