src/lean/Pod/Storable.lean
@@ -1,0 +1,116 @@
+import Pod.Lemmas
+
+namespace Pod
+
+class Storable (α : Type) where
+  byteSize : USize
+  byteSize_gt_zero : byteSize.toNat > 0
+  alignment : Nat
+  alignment_dvd_byteSize : ∃ k, byteSize.toNat = alignment * k
+
+export Storable (byteSize byteSize_gt_zero alignment alignment_dvd_byteSize)
+
+theorem not_alignment_eq_zero {α} [Storable α] : ¬ alignment α = 0 := by
+    intro h
+    apply Nat.not_eq_zero_of_lt $ byteSize_gt_zero (α := α)
+    apply (@alignment_dvd_byteSize α).elim
+    intro k b
+    rw [b, h]
+    exact Nat.zero_mul k
+
+def bitWidth {α} [Storable α] : USize := byteSize α * 8
+
+instance : Storable UInt8 where
+  byteSize := 1
+  byteSize_gt_zero := Nat.lt_of_lt_of_eq (by constructor) (mod_usize_size_eq 1 $ by decide).symm
+  alignment := 1
+  alignment_dvd_byteSize := Exists.intro 1 (mod_usize_size_eq 1 $ by decide)
+
+instance : Storable UInt16 where
+  byteSize := 2
+  byteSize_gt_zero := Nat.lt_of_lt_of_eq (by decide) (mod_usize_size_eq 2 $ by decide).symm
+  alignment := 2
+  alignment_dvd_byteSize := Exists.intro 1 (mod_usize_size_eq 2 $ by decide)
+
+instance : Storable UInt32 where
+  byteSize := 4
+  byteSize_gt_zero := Nat.lt_of_lt_of_eq (by decide) (mod_usize_size_eq 4 $ by decide).symm
+  alignment := 4
+  alignment_dvd_byteSize := Exists.intro 1 (mod_usize_size_eq 4 $ by decide)
+
+@[extern "lean_pod_UInt64_getAlignment"]
+private
+opaque UInt64.getAlignment : @& Unit → { n : Nat // n = 4 ∨ n = 8 } := λ _ ↦ ⟨8, Or.inr rfl⟩
+
+instance : Storable UInt64 where
+  byteSize := 8
+  byteSize_gt_zero := Nat.lt_of_lt_of_eq (by decide) (mod_usize_size_eq 8 $ by decide).symm
+  alignment := (UInt64.getAlignment ()).val
+  alignment_dvd_byteSize := match (UInt64.getAlignment ()).property with
+    | Or.inl h => Exists.intro 2 $ by show 8 % USize.size = _; rw [h, mod_usize_size_eq 8 $ by decide]
+    | Or.inr h => Exists.intro 1 $ by show 8 % USize.size = _; rw [h, mod_usize_size_eq 8 $ by decide]
+
+theorem alignment_UInt64_eq : alignment UInt64 = 4 ∨ alignment UInt64 = 8 :=
+  (UInt64.getAlignment ()).property
+
+instance : Storable USize where
+  byteSize := if System.Platform.numBits = 32 then byteSize UInt32 else byteSize UInt64
+  byteSize_gt_zero := match System.Platform.numBits, System.Platform.numBits_eq with
+    | 32, Or.inl _ => byteSize_gt_zero
+    | 64, Or.inr _ => byteSize_gt_zero
+  alignment := if System.Platform.numBits = 32 then alignment UInt32 else alignment UInt64
+  alignment_dvd_byteSize := match System.Platform.numBits, System.Platform.numBits_eq with
+    | 32, Or.inl _ => alignment_dvd_byteSize
+    | 64, Or.inr _ => alignment_dvd_byteSize
+
+@[extern "lean_pod_Float_getAlignment"]
+private
+opaque Float.getAlignment : @& Unit → { n : Nat // n = 4 ∨ n = 8 } := λ _ ↦ ⟨8, Or.inr rfl⟩
+
+instance : Storable Float where
+  byteSize := 8
+  byteSize_gt_zero := Nat.lt_of_lt_of_eq (by decide) (mod_usize_size_eq 8 $ by decide).symm
+  alignment := (Float.getAlignment ()).val
+  alignment_dvd_byteSize := match (Float.getAlignment ()).property with
+    | Or.inl h => Exists.intro 2 $ by show 8 % USize.size = _; rw [h, mod_usize_size_eq 8 $ by decide]
+    | Or.inr h => Exists.intro 1 $ by show 8 % USize.size = _; rw [h, mod_usize_size_eq 8 $ by decide]
+
+theorem alignment_Float_eq : alignment Float = 4 ∨ alignment Float = 8 :=
+  (Float.getAlignment ()).property
+
+theorem offEl_no_overflow {α size} [Storable α] (i : USize)
+  (h : i.toNat * (byteSize α).toNat + (byteSize α).toNat ≤ USize.toNat size) :
+    (i * byteSize α).toNat = i.toNat * (byteSize α).toNat := by
+      apply Nat.mod_eq_of_lt
+      apply Nat.lt_of_le_of_lt
+      · show i.toNat * (byteSize α).toNat + 0 ≤ i.toNat * (byteSize α).toNat + (byteSize α).toNat
+        apply Nat.add_le_add_left
+        exact Nat.zero_le _
+      · exact Nat.lt_of_le_of_lt h size.val.isLt
+
+theorem offEl_aligned {α size} [Storable α] (i : USize)
+  (h : i.toNat * (byteSize α).toNat + (byteSize α).toNat ≤ USize.toNat size) :
+  ∀ m, ∃ n, alignment α * m + (i * byteSize α).toNat = (alignment α) * n := λ m ↦
+    (alignment_dvd_byteSize (α := α)).elim λ aib h₁ ↦
+      Exists.intro (m + i.toNat * aib) $ by
+        rewrite [Nat.left_distrib]
+        apply congrArg (alignment α * m + ·)
+        rewrite [Nat.mul_comm _ aib, ← Nat.mul_assoc, ← h₁, Nat.mul_comm]
+        rw [offEl_no_overflow i h]
+
+theorem off_lt_usize_size {α size} [Storable α] (i : Nat) (h : i + (byteSize α).toNat ≤ USize.toNat size) :
+  i < USize.size := calc
+    i ≤ i + (byteSize α).toNat := Nat.add_le_add_left (Nat.zero_le _) i
+    _ ≤ size.toNat             := h
+    _ < USize.size             := size.val.isLt
+
+theorem offEl_lt_usize_size {α size} [Storable α] (i : Nat)
+  (h : i * (byteSize α).toNat + (byteSize α).toNat ≤ USize.toNat size) :
+    i < USize.size := calc
+      i = i * 1                                       := Eq.symm (Nat.mul_one i)
+      _ ≤ i * (byteSize α).toNat + 0                  := Nat.mul_le_mul_left i byteSize_gt_zero
+      _ ≤ i * (byteSize α).toNat + (byteSize α).toNat := Nat.add_le_add_left (Nat.zero_le _) _
+      _ ≤ size.toNat                                  := h
+      _ < USize.size                                  := size.val.isLt
+
+end Pod
