src/lean/Pod/WriteBytes.lean
@@ -1,0 +1,67 @@
+import Pod.Storable
+import Pod.BytesRef
+
+namespace Pod
+
+class WriteBytes (α : Type) extends Storable α where
+  writeBytesRefOffUnal {σ size align} : BytesRefMut σ size align → (i : USize) →
+    i.toNat + byteSize.toNat ≤ size.toNat → α → ST σ Unit
+
+  writeBytesRefUnal {σ align} (br : BytesRefMut σ byteSize align) : α → ST σ Unit :=
+    writeBytesRefOffUnal br 0 (Nat.le_of_eq $ Nat.zero_add _)
+
+  writeBytesRefOffElUnal {σ size align} (br : BytesRefMut σ size align) (i : USize)
+    (h : i.toNat * byteSize.toNat + byteSize.toNat ≤ size.toNat) : α → ST σ Unit :=
+      writeBytesRefOffUnal br (i * byteSize) (by rw [offEl_no_overflow i h]; exact h)
+
+  writeBytesRefOff {σ size align} : BytesRefMut σ size align → (i : USize) →
+    i.toNat + byteSize.toNat ≤ size.toNat →
+    (∀ m, ∃ n, align * m + i.toNat = alignment * n) → α → ST σ Unit
+
+  writeBytesRef {σ} (br : BytesRefMut σ byteSize alignment) : α → ST σ Unit :=
+    writeBytesRefOff br 0 (Nat.le_of_eq $ Nat.zero_add _) λ m ↦
+      Exists.intro m (by rw [Nat.add_comm]; exact Nat.zero_add _)
+
+  writeBytesRefOffEl {σ size} (br : BytesRefMut σ size alignment) (i : USize)
+    (h : i.toNat * byteSize.toNat + byteSize.toNat ≤ size.toNat) : α → ST σ Unit :=
+      writeBytesRefOff br (i * byteSize) (by rw [offEl_no_overflow i h]; exact h) (offEl_aligned i h)
+
+def BytesRef.setUnal {α σ align} [WriteBytes α] (br : BytesRefMut σ (byteSize α) align) (value : α) : ST σ Unit :=
+  WriteBytes.writeBytesRefUnal br value
+
+def BytesRef.usetOffUnal {α σ size align} [WriteBytes α] (br : BytesRefMut σ size align) (i : USize)
+  (h₁ : i.toNat + (byteSize α).toNat ≤ size.toNat) (value : α) : ST σ Unit :=
+    WriteBytes.writeBytesRefOffUnal br i h₁ value
+
+def BytesRef.setOffUnal {α σ size align} [WriteBytes α] (br : BytesRefMut σ size align) (i : Nat)
+  (h₁ : i + (byteSize α).toNat ≤ size.toNat) (value : α) : ST σ Unit :=
+    WriteBytes.writeBytesRefOffUnal br ⟨i, off_lt_usize_size i h₁⟩ h₁ value
+
+def BytesRef.usetOffElUnal {α σ size align} [WriteBytes α] (br : BytesRefMut σ size align)
+  (i : USize) (h : i.toNat * (byteSize α).toNat + (byteSize α).toNat ≤ size.toNat) (value : α) : ST σ Unit :=
+    WriteBytes.writeBytesRefOffElUnal br i h value
+
+def BytesRef.setOffElUnal {α σ size align} [WriteBytes α] (br : BytesRefMut σ size align)
+  (i : Nat) (h : i * (byteSize α).toNat + (byteSize α).toNat ≤ size.toNat) (value : α) : ST σ Unit :=
+    WriteBytes.writeBytesRefOffElUnal br ⟨i, offEl_lt_usize_size i h⟩ h value
+
+def BytesRef.set {α σ} [WriteBytes α] (br : BytesRefMut σ (byteSize α) (alignment α)) (value : α) : ST σ Unit :=
+  WriteBytes.writeBytesRef br value
+
+def BytesRef.usetOff {α σ size align} [WriteBytes α] (br : BytesRefMut σ size align) (i : USize)
+  (h₁ : i.toNat + (byteSize α).toNat ≤ size.toNat)
+  (h₂ : ∀ m, ∃ n, align * m + i.toNat = alignment α * n) (value : α) : ST σ Unit :=
+    WriteBytes.writeBytesRefOff br i h₁ h₂ value
+
+def BytesRef.setOff {α σ size align} [WriteBytes α] (br : BytesRefMut σ size align) (i : Nat)
+  (h₁ : i + (byteSize α).toNat ≤ size.toNat)
+  (h₂ : ∀ m, ∃ n, align * m + i = alignment α * n) (value : α) : ST σ Unit :=
+    WriteBytes.writeBytesRefOff br ⟨i, off_lt_usize_size i h₁⟩ h₁ h₂ value
+
+def BytesRef.usetOffEl {α σ size} [WriteBytes α] (br : BytesRefMut σ size (alignment α))
+  (i : USize) (h : i.toNat * (byteSize α).toNat + (byteSize α).toNat ≤ size.toNat) (value : α) : ST σ Unit :=
+    WriteBytes.writeBytesRefOffEl br i h value
+
+def BytesRef.setOffEl {α σ size} [WriteBytes α] (br : BytesRefMut σ size (alignment α))
+  (i : Nat) (h : i * (byteSize α).toNat + (byteSize α).toNat ≤ size.toNat) (value : α) : ST σ Unit :=
+    WriteBytes.writeBytesRefOffEl br ⟨i, offEl_lt_usize_size i h⟩ h value
